theories/Translations/LustreToTiming.v
@@ -37,7 +37,7 @@ Fixpoint expr_to_raw {ty} (e: Lustre.exp ty): LustreTiming.raw_exp ty :=
       end (expr_to_raw e1) (expr_to_raw e2)
   end.
 
-Definition translate_expr_aux {ty} (e: Lustre.exp ty) (ident_origin: ident) (pre_binders: list LustreTiming.binder) (pre_equations init_post_equations step_post_equations: list LustreTiming.equation): (
+Definition translate_expr {ty} (e: Lustre.exp ty) (ident_origin: ident) (pre_binders: list LustreTiming.binder) (pre_equations init_post_equations step_post_equations: list LustreTiming.equation): (
     LustreTiming.comb_exp ty (* init *)
     * LustreTiming.comb_exp ty (* step *)
     * ident (* New identifier origin *)
@@ -54,8 +54,15 @@ Definition translate_expr_aux {ty} (e: Lustre.exp ty) (ident_origin: ident) (pre
     * (list LustreTiming.equation) (* init_post equations *)
     * (list LustreTiming.equation) (* step_post equations *)
   ) :=
-    LustreTiming.raw_to_comb_aux (expr_to_raw e) ident_origin pre_binders pre_equations init_post_equations step_post_equations.
+    LustreTiming.raw_to_comb (expr_to_raw e) ident_origin pre_binders pre_equations init_post_equations step_post_equations.
 
+Lemma freshness_translate_expr {ty} {e: Lustre.exp ty} {ei es: LustreTiming.comb_exp ty} {seed0 seed1: ident} {binders pre_binders0 pre_binders1: list LustreTiming.binder} {pre_eqs0 pre_eqs1 init_post0 init_post1 step_post0 step_post1: list LustreTiming.equation}:
+  translate_expr e seed0 pre_binders0 pre_eqs0 init_post0 step_post0 = (ei, es, seed1, pre_binders1, pre_eqs1, init_post1, step_post1)
+  -> LustreTiming.freshness seed0 (pre_binders0 ++ binders)
+  -> LustreTiming.freshness seed1 (pre_binders1 ++ binders).
+Proof.
+  apply LustreTiming.freshness_raw_to_comb.
+Qed.
 
 Fixpoint translate_equations (eqs: list Lustre.equation) (ident_origin: ident): (
     list LustreTiming.equation (* init *)
@@ -138,11 +145,11 @@ Proof.
 
   all: subst n_vars n_assigned_vars.
 
-  - clear -translation n_vars_all_assigned n_vars_unique.
+  - clear -translation n_vars_all_assigned n_vars_unique n_seed_always_fresh.
 
     apply NoDup_map_inv in n_vars_unique.
 
-    induction n_body as [ | eq n_body IHn] in translation, n_vars_unique, init_eqs, step_eqs, new_seed, pre_binders, pre_eqs, init_post_eqs, step_post_eqs, n_seed, n_vars_all_assigned, n_out, n_locals |- *.
+    induction n_body as [ | eq n_body IHn] in translation, n_vars_unique, init_eqs, step_eqs, new_seed, pre_binders, pre_eqs, init_post_eqs, step_post_eqs, n_seed, n_vars_all_assigned, n_out, n_locals, n_seed_always_fresh |- *.
     + unfold translate_equations in translation.
       injection translation as <- <- <- <- <- <- <-.
       simpl.
@@ -153,7 +160,7 @@ Proof.
     + destruct eq as [eq_ident [ty eq_expr]].
       cbn in translation.
       destruct (translate_equations n_body n_seed) as [[[[[[init_eqs0 step_eqs0] new_seed_0] pre_binders0] pre_eqs0] init_post_eqs0] step_post_eqs0] eqn: eq_trans_eq.
-      destruct (@translate_expr_aux ty eq_expr new_seed_0 pre_binders0 pre_eqs0 init_post_eqs0 step_post_eqs0) as [[[[[[ei es] new_seed_bis] binders] equations_pre] init_equations_post] step_equations_post] eqn: eqe.
+      destruct (@translate_expr ty eq_expr new_seed_0 pre_binders0 pre_eqs0 init_post_eqs0 step_post_eqs0) as [[[[[[ei es] new_seed_bis] binders] equations_pre] init_equations_post] step_equations_post] eqn: eqe.
       injection translation as <- <- <- <- <- <- <-.
 
       rewrite map_cons in n_vars_all_assigned.
@@ -163,98 +170,131 @@ Proof.
       rewrite map_cons.
       unfold LustreTiming.equation_dest at 2, fst, snd, projT1.
 
-      specialize (IHn [] (map Lustre.equation_dest n_body)).
-      simpl in IHn.
-      specialize (IHn (Permutation_refl (map Lustre.equation_dest n_body))).
-
-      assert (nodup_IH := n_vars_unique).
-      rewrite (Permutation_sym n_vars_all_assigned) in nodup_IH.
-
-      assert (nodup_2 := nodup_IH).
-      apply NoDup_app_remove_l in nodup_2.
-      apply (permutation_nodup_remove_cons Lustre.binder_dec _ _ _ n_vars_all_assigned) in nodup_2.
-
-      apply NoDup_remove_1 in nodup_IH.
-      specialize (IHn nodup_IH _ _ _ _ _ _ _ _ eq_trans_eq).
-      clear nodup_IH.
-
-      rewrite map_app in IHn.
-      rewrite nodup_2 in IHn.
-
       assert (eq_in_out_locals := n_vars_all_assigned).
 
       apply (Permutation_in (eq_ident, ty)) in eq_in_out_locals.
       2: left; reflexivity.
 
-      assert (nodup_out_locals := NoDup_app_remove_l _ _ n_vars_unique).
+      assert (nodup_out_locals := n_vars_unique).
 
-      assert (
-        permut_add_out := add_removed Lustre.binder_dec _ _ eq_in_out_locals nodup_out_locals
-      ).
-      clear eq_in_out_locals nodup_out_locals.
+      apply NoDup_app_remove_l in nodup_out_locals.
 
-      rewrite (Permutation_app_comm binders n_locals).
-      simpl.
-      rewrite app_assoc.
-      rewrite permut_add_out.
+      assert (vars_assigned_removed := permutation_nodup_remove_cons Lustre.binder_dec _ _ _ n_vars_all_assigned (Permutation_NoDup (Permutation_sym n_vars_all_assigned) nodup_out_locals)).
+      rewrite remove_app in vars_assigned_removed.
+
       simpl.
       rewrite <- Permutation_middle.
 
-      apply perm_skip.
-      
-      rewrite (Permutation_app_comm _ binders).
+      specialize (IHn _ _ vars_assigned_removed).
 
-      clear -eqe IHn.
+      assert (vars_unique_remove := NoDup_app_list_remove_r Lustre.binder_dec (eq_ident, ty) _ _ n_vars_unique).
+      rewrite remove_app in vars_unique_remove.
 
-      revert eqe.
+      specialize (IHn vars_unique_remove).
 
-      induction eq_expr.
-      all: intro eqe.
-      * unfold translate_expr_aux in eqe.
+      assert (fresh_remove : forall n : nat,
+              ~In (iter n next_ident n_seed)
+              (map fst (n_in ++
+              remove Lustre.binder_dec (eq_ident, ty) n_out ++
+              remove Lustre.binder_dec (eq_ident, ty) n_locals))
+      ).
+      1: intro n.
+      1: specialize (n_seed_always_fresh n).
+      1: apply (remove_map_notinr Lustre.binder_dec (eq_ident, ty)) in n_seed_always_fresh.
+      1: rewrite remove_app in n_seed_always_fresh.
+      1: assumption.
+
+      specialize (IHn _ fresh_remove).
+      specialize (IHn _ _ _ _ _ _ _ eq_trans_eq).
+
+      clear -IHn eqe eq_in_out_locals nodup_out_locals fresh_remove eq_in_out_locals.
+
+      induction eq_expr in n_in, n_out, n_locals, eq_ident, n_seed, init_eqs0, new_seed_0, pre_binders0, pre_eqs0, init_post_eqs0, step_post_eqs0, ei, es, new_seed_bis, binders, equations_pre, init_equations_post, step_equations_post, eqe, IHn, eq_in_out_locals, nodup_out_locals, fresh_remove, eq_in_out_locals |- *.
+      * unfold translate_expr in eqe.
         simpl in eqe.
         injection eqe as <- <- <- <- <- <- <-.
+        rewrite map_app in IHn.
+        apply Permutation_sym in IHn.
+        rewrite Permutation_app_comm in IHn.
+        rewrite <- app_assoc in IHn.
+        rewrite <- remove_app in IHn.
+        apply Permutation_sym in IHn.
+        rewrite (Permutation_app_comm n_out).
+        rewrite <- app_assoc.
+        apply (perm_skip (eq_ident, ty)) in IHn.
+        rewrite IHn.
+        rewrite Permutation_app_comm.
+        rewrite (Permutation_app_comm pre_binders0).
+        apply (Permutation_app_tail (l:=_ :: _)).
+        apply Permutation_sym.
+        apply add_removed.
+        1: apply In_app_inv; assumption.
+        apply NoDup_app_inv.
         assumption.
-      * unfold translate_expr_aux in eqe.
+      * unfold translate_expr in eqe.
         simpl in eqe.
         injection eqe as <- <- <- <- <- <- <-.
+        rewrite map_app in IHn.
+        apply Permutation_sym in IHn.
+        rewrite Permutation_app_comm in IHn.
+        rewrite <- app_assoc in IHn.
+        rewrite <- remove_app in IHn.
+        apply Permutation_sym in IHn.
+        rewrite (Permutation_app_comm n_out).
+        rewrite <- app_assoc.
+        apply (perm_skip (eq_ident, Lustre.binder_ty b)) in IHn.
+        rewrite IHn.
+        rewrite Permutation_app_comm.
+        rewrite (Permutation_app_comm pre_binders0).
+        apply (Permutation_app_tail (l:=_ :: _)).
+        apply Permutation_sym.
+        apply add_removed.
+        1: apply In_app_inv; assumption.
+        apply NoDup_app_inv.
         assumption.
       * destruct u.
-        -- unfold translate_expr_aux in eqe.
+        -- unfold translate_expr in eqe.
            simpl in eqe.
-           destruct (@LustreTiming.raw_to_comb_aux LustreTiming.TInt (@expr_to_raw Lustre.TInt eq_expr) new_seed_0 pre_binders0 pre_eqs0 init_post_eqs0 step_post_eqs0) as [[[[[[ei1 es1] new_seed_1] pre_binders1] pre_eqs1] init_post_eqs1] step_post_eqs1] eqn: unfold1.
+           destruct (@LustreTiming.raw_to_comb LustreTiming.TInt (@expr_to_raw Lustre.TInt eq_expr) new_seed_0 pre_binders0 pre_eqs0 init_post_eqs0 step_post_eqs0) as [[[[[[ei1 es1] new_seed_bis1] binders1] equations_pre1] init_equations_post1] step_equations_post1] eqn: eqe1.
            injection eqe as <- <- <- <- <- <- <-.
-           specialize (IHeq_expr _ _ IHn unfold1).
-           assumption.
-        -- unfold translate_expr_aux in eqe.
+
+           specialize (IHeq_expr _ _ _ _ _ _ _ _ _ _ _ _ _ _ _ _ _ _ eqe1 IHn eq_in_out_locals nodup_out_locals fresh_remove).
+           exact IHeq_expr.
+        -- unfold translate_expr in eqe.
            simpl in eqe.
-           destruct (@LustreTiming.raw_to_comb_aux LustreTiming.TInt (@expr_to_raw Lustre.TInt eq_expr) new_seed_0 pre_binders0 pre_eqs0 init_post_eqs0 step_post_eqs0) as [[[[[[ei1 es1] new_seed_1] pre_binders1] pre_eqs1] init_post_eqs1] step_post_eqs1] eqn: unfold1.
+           destruct (@LustreTiming.raw_to_comb LustreTiming.TInt (@expr_to_raw Lustre.TInt eq_expr) new_seed_0 pre_binders0 pre_eqs0 init_post_eqs0 step_post_eqs0) as [[[[[[ei1 es1] new_seed_bis1] binders1] equations_pre1] init_equations_post1] step_equations_post1] eqn: eqe1.
            injection eqe as <- <- <- <- <- <- <-.
-           specialize (IHeq_expr _ _ IHn unfold1).
-           assumption.
-        -- unfold translate_expr_aux in eqe.
+
+           specialize (IHeq_expr _ _ _ _ _ _ _ _ _ _ _ _ _ _ _ _ _ _ eqe1 IHn eq_in_out_locals nodup_out_locals fresh_remove).
+           exact IHeq_expr.
+        -- unfold translate_expr in eqe.
            simpl in eqe.
-           destruct (@LustreTiming.raw_to_comb_aux Lustre.TInt (@expr_to_raw Lustre.TInt eq_expr) new_seed_0 pre_binders0 pre_eqs0 init_post_eqs0 step_post_eqs0) as [[[[[[ei1 es1] new_seed_1] pre_binders1] pre_eqs1] init_post_eqs1] step_post_eqs1] eqn: unfold1.
+           destruct (@LustreTiming.raw_to_comb Lustre.TInt (@expr_to_raw Lustre.TInt eq_expr) new_seed_0 pre_binders0 pre_eqs0 init_post_eqs0 step_post_eqs0) as [[[[[[ei1 es1] new_seed_bis1] binders1] equations_pre1] init_equations_post1] step_equations_post1] eqn: eqe1.
            injection eqe as <- <- <- <- <- <- <-.
+
+           specialize (IHeq_expr _ _ _ _ _ _ _ _ _ _ _ _ _ _ _ _ _ _ eqe1 IHn eq_in_out_locals nodup_out_locals fresh_remove).
 
            simpl.
-           unfold LustreTiming.equation_dest at 1 4, fst, snd, projT1.
-           simpl in IHeq_expr.
-           unfold LustreTiming.equation_dest at 4 7, fst, snd, projT1 in IHeq_expr.
-           eapply IHeq_expr.
-           1: assumption.
-           unfold translate_expr_aux.
-           rewrite unfold1.
-           split.
-      * destruct b.
-        -- unfold translate_expr_aux in eqe.
-           simpl in eqe.
-           destruct (@LustreTiming.raw_to_comb_aux LustreTiming.TBool (@expr_to_raw Lustre.TBool eq_expr1) new_seed_0 pre_binders0 pre_eqs0 init_post_eqs0 step_post_eqs0) as [[[[[[ei1 es1] new_seed_1] pre_binders1] pre_eqs1] init_post_eqs1] step_post_eqs1] eqn: unfold1.
-           destruct (@LustreTiming.raw_to_comb_aux LustreTiming.TBool (@expr_to_raw Lustre.TBool eq_expr2) new_seed_1 pre_binders1 pre_eqs1 init_post_eqs1 step_post_eqs1) as [[[[[[ei2 es2] new_seed_2] pre_binders2] pre_eqs2] init_post_eqs2] step_post_eqs2] eqn: unfold2.
-           injection eqe as <- <- <- <- <- <- <-.
-           specialize (IHeq_expr1 _ _ IHn unfold1).
-           
 
-      Search Permutation app.
+           unfold LustreTiming.equation_dest at 1 4, fst, snd, projT1.
+
+           apply (Permutation_elt [_] _ n_out).
+           simpl.
+
+           (* TODO LATER FLEMME *)
+           apply ABORT_FIXME; exact tt.
+      * destruct b.
+        -- unfold translate_expr in eqe.
+           simpl in eqe.
+           destruct (@LustreTiming.raw_to_comb LustreTiming.TBool (@expr_to_raw Lustre.TBool eq_expr1) new_seed_0 pre_binders0 pre_eqs0 init_post_eqs0 step_post_eqs0) as [[[[[[ei1 es1] new_seed_bis1] binders1] equations_pre1] init_equations_post1] step_equations_post1] eqn: eqe1.
+           destruct (@LustreTiming.raw_to_comb LustreTiming.TBool (@expr_to_raw Lustre.TBool eq_expr2) new_seed_bis1 binders1 equations_pre1 init_equations_post1 step_equations_post1) as [[[[[[ei2 es2] new_seed_bis2] binders2] equations_pre2] init_equations_post2] step_equations_post2] eqn: eqe2.
+           injection eqe as <- <- <- <- <- <- <-.
+
+           specialize (IHeq_expr1 _ _ _ _ _ _ _ _ _ _ _ _ _ _ _ _ _ _ eqe1 IHn eq_in_out_locals nodup_out_locals fresh_remove).
+           rewrite <- map_app in IHeq_expr1.
+           apply (perm_remove_app_without_mid Lustre.binder_dec _ _ _ _ _ _ eq_in_out_locals) in IHeq_expr1.
+           specialize (IHeq_expr2 _ _ _ _ _ _ _ _ _ _ _ _ _ _ _ _ _ _ eqe2 IHeq_expr1 eq_in_out_locals nodup_out_locals fresh_remove).
+           exact IHeq_expr.
     (*
     assert (H := n_vars_all_assigned).
       rewrite map_cons in H.
@@ -266,7 +306,7 @@ Proof.
       specialize (IHn_body incl_nbody _ _ _ _ _ _ _ _ eqIh).
       unfold Lustre.equation_dest, fst, snd, projT1 in ina.
       clear -translation IHn_body ina.
-      destruct (translate_expr_aux e new_ident_origin0 pre_binders0 pre_eqs0 init_post_eqs0 step_post_eqs0) as [[[[[[ei es] orig] binders] equations_pre] init_equations_post] step_equations_post] eqn: eqe.
+      destruct (translate_expr e new_ident_origin0 pre_binders0 pre_eqs0 init_post_eqs0 step_post_eqs0) as [[[[[[ei es] orig] binders] equations_pre] init_equations_post] step_equations_post] eqn: eqe.
       injection translation as <- <- <- <- <- <- <-.
 
       simpl.
@@ -290,10 +330,10 @@ Proof.
         assumption.
       * simpl.
         destruct u.
-        all: unfold translate_expr_aux in eqe.
+        all: unfold translate_expr in eqe.
         all: simpl in eqe.
-        1-2: destruct (@LustreTiming.raw_to_comb_aux LustreTiming.TInt (@expr_to_raw Lustre.TInt e) new_ident_origin0 pre_binders0 pre_eqs0 init_post_eqs0 step_post_eqs0) as [[[[[[]]]]]] eqn: e_unfold.
-        3: destruct (@LustreTiming.raw_to_comb_aux Lustre.TInt (@expr_to_raw Lustre.TInt e) new_ident_origin0 pre_binders0 pre_eqs0 init_post_eqs0 step_post_eqs0) as [[[[[[]]]]]] eqn: e_unfold.
+        1-2: destruct (@LustreTiming.raw_to_comb LustreTiming.TInt (@expr_to_raw Lustre.TInt e) new_ident_origin0 pre_binders0 pre_eqs0 init_post_eqs0 step_post_eqs0) as [[[[[[]]]]]] eqn: e_unfold.
+        3: destruct (@LustreTiming.raw_to_comb Lustre.TInt (@expr_to_raw Lustre.TInt e) new_ident_origin0 pre_binders0 pre_eqs0 init_post_eqs0 step_post_eqs0) as [[[[[[]]]]]] eqn: e_unfold.
         all: injection eqe as <- <- <- <- <- <- <-.
         1-2: refine (IHe _ _ _ _ _ _ _ _ _ _ _ _ _ _ _ _ e_unfold IHn_body).
         simpl.
@@ -328,17 +368,17 @@ Proof.
               apply incl_refl.
       * simpl.
         destruct b.
-        all: unfold translate_expr_aux in eqe.
+        all: unfold translate_expr in eqe.
         all: simpl in eqe.
-        1-3: destruct (@LustreTiming.raw_to_comb_aux LustreTiming.TBool (@expr_to_raw Lustre.TBool e1) new_ident_origin0 pre_binders0 pre_eqs0 init_post_eqs0 step_post_eqs0) as [[[[[[c1 c2] ident_e1] binders_e1] eqs_e1] init_e1] step_e1] eqn: e1_unfold.
-        1-3: destruct (@LustreTiming.raw_to_comb_aux LustreTiming.TBool (@expr_to_raw Lustre.TBool e2) ident_e1 binders_e1 eqs_e1 init_e1 step_e1) as [[[[[[]]]]]] eqn: e2_unfold.
-        4-13: destruct (@LustreTiming.raw_to_comb_aux LustreTiming.TInt (@expr_to_raw Lustre.TInt e1) new_ident_origin0 pre_binders0 pre_eqs0 init_post_eqs0 step_post_eqs0) as [[[[[[c1 c2] ident_e1] binders_e1] eqs_e1] init_e1] step_e1] eqn: e1_unfold.
-        4-13: destruct (@LustreTiming.raw_to_comb_aux LustreTiming.TInt (@expr_to_raw Lustre.TInt e2) ident_e1 binders_e1 eqs_e1 init_e1 step_e1) as [[[[[[]]]]]] eqn: e2_unfold.
+        1-3: destruct (@LustreTiming.raw_to_comb LustreTiming.TBool (@expr_to_raw Lustre.TBool e1) new_ident_origin0 pre_binders0 pre_eqs0 init_post_eqs0 step_post_eqs0) as [[[[[[c1 c2] ident_e1] binders_e1] eqs_e1] init_e1] step_e1] eqn: e1_unfold.
+        1-3: destruct (@LustreTiming.raw_to_comb LustreTiming.TBool (@expr_to_raw Lustre.TBool e2) ident_e1 binders_e1 eqs_e1 init_e1 step_e1) as [[[[[[]]]]]] eqn: e2_unfold.
+        4-13: destruct (@LustreTiming.raw_to_comb LustreTiming.TInt (@expr_to_raw Lustre.TInt e1) new_ident_origin0 pre_binders0 pre_eqs0 init_post_eqs0 step_post_eqs0) as [[[[[[c1 c2] ident_e1] binders_e1] eqs_e1] init_e1] step_e1] eqn: e1_unfold.
+        4-13: destruct (@LustreTiming.raw_to_comb LustreTiming.TInt (@expr_to_raw Lustre.TInt e2) ident_e1 binders_e1 eqs_e1 init_e1 step_e1) as [[[[[[]]]]]] eqn: e2_unfold.
         1-13: injection eqe as <- <- <- <- <- <- <-.
         1-13: refine (IHe2 _ _ _ _ _ _ _ _ _ _ _ _ _ _ _ _ e2_unfold (IHe1 _ _ _ _ _ _ _ _ _ _ _ _ _ _ _ _ e1_unfold IHn_body)).
 
-        destruct (@LustreTiming.raw_to_comb_aux Lustre.TInt (@expr_to_raw Lustre.TInt e1) new_ident_origin0 pre_binders0 pre_eqs0 init_post_eqs0 step_post_eqs0) as [[[[[[c1 c2] ident_e1] binders_e1] eqs_e1] init_e1] step_e1] eqn: e1_unfold.
-        destruct (@LustreTiming.raw_to_comb_aux Lustre.TInt (@expr_to_raw Lustre.TInt e2) ident_e1 binders_e1 eqs_e1 init_e1 step_e1) as [[[[[[]]]]]] eqn: e2_unfold.
+        destruct (@LustreTiming.raw_to_comb Lustre.TInt (@expr_to_raw Lustre.TInt e1) new_ident_origin0 pre_binders0 pre_eqs0 init_post_eqs0 step_post_eqs0) as [[[[[[c1 c2] ident_e1] binders_e1] eqs_e1] init_e1] step_e1] eqn: e1_unfold.
+        destruct (@LustreTiming.raw_to_comb Lustre.TInt (@expr_to_raw Lustre.TInt e2) ident_e1 binders_e1 eqs_e1 init_e1 step_e1) as [[[[[[]]]]]] eqn: e2_unfold.
         injection eqe as <- <- <- <- <- <- <-.
         simpl.
         specialize (IHe2 _ _ _ _ _ _ _ _ _ _ _ _ _ _ _ _ e2_unfold (IHe1 _ _ _ _ _ _ _ _ _ _ _ _ _ _ _ _ e1_unfold IHn_body)).
@@ -356,11 +396,11 @@ Proof.
         ++ apply incl_app_inv in IHe2.
           destruct IHe2 as [_ incl_l1].
           apply incl_l1.
-      * unfold translate_expr_aux in eqe.
+      * unfold translate_expr in eqe.
         simpl in eqe.
-        destruct (@LustreTiming.raw_to_comb_aux LustreTiming.TBool (@expr_to_raw Lustre.TBool e1) new_ident_origin0 pre_binders0 pre_eqs0 init_post_eqs0 step_post_eqs0) as [[[[[[? ?] ident_e1] binders_e1] eqs_e1] init_e1] step_e1] eqn: e1_unfold.
-        destruct (@LustreTiming.raw_to_comb_aux t (@expr_to_raw t e2) ident_e1 binders_e1 eqs_e1 init_e1 step_e1) as [[[[[[? ?] ident_e2] binders_e2] eqs_e2] init_e2] step_e2] eqn: e2_unfold.
-        destruct (@LustreTiming.raw_to_comb_aux t (@expr_to_raw t e3) ident_e2 binders_e2 eqs_e2 init_e2 step_e2) as [[[[[[]]]]]] eqn: e3_unfold.
+        destruct (@LustreTiming.raw_to_comb LustreTiming.TBool (@expr_to_raw Lustre.TBool e1) new_ident_origin0 pre_binders0 pre_eqs0 init_post_eqs0 step_post_eqs0) as [[[[[[? ?] ident_e1] binders_e1] eqs_e1] init_e1] step_e1] eqn: e1_unfold.
+        destruct (@LustreTiming.raw_to_comb t (@expr_to_raw t e2) ident_e1 binders_e1 eqs_e1 init_e1 step_e1) as [[[[[[? ?] ident_e2] binders_e2] eqs_e2] init_e2] step_e2] eqn: e2_unfold.
+        destruct (@LustreTiming.raw_to_comb t (@expr_to_raw t e3) ident_e2 binders_e2 eqs_e2 init_e2 step_e2) as [[[[[[]]]]]] eqn: e3_unfold.
         injection eqe as <- <- <- <- <- <- <-.
         refine (IHe3 _ _ _ _ _ _ _ _ _ _ _ _ _ _ _ _ e3_unfold (IHe2 _ _ _ _ _ _ _ _ _ _ _ _ _ _ _ _ e2_unfold (IHe1 _ _ _ _ _ _ _ _ _ _ _ _ _ _ _ _ e1_unfold IHn_body))). *)
   - apply ABORT_FIXME; exact tt.
@@ -380,7 +420,7 @@ Proof.
       specialize (IHn_body incl_nbody _ _ _ _ _ _ _ _ eqIh).
       unfold Lustre.equation_dest, fst, snd, projT1 in ina.
       clear -translation IHn_body ina.
-      destruct (translate_expr_aux e new_ident_origin0 pre_binders0 pre_eqs0 init_post_eqs0 step_post_eqs0) as [[[[[[ei es] orig] binders] equations_pre] init_equations_post] step_equations_post] eqn: eqe.
+      destruct (translate_expr e new_ident_origin0 pre_binders0 pre_eqs0 init_post_eqs0 step_post_eqs0) as [[[[[[ei es] orig] binders] equations_pre] init_equations_post] step_equations_post] eqn: eqe.
       injection translation as <- <- <- <- <- <- <-.
 
       simpl.
@@ -397,10 +437,10 @@ Proof.
         assumption.
       * simpl.
         destruct u.
-        all: unfold translate_expr_aux in eqe.
+        all: unfold translate_expr in eqe.
         all: simpl in eqe.
-        1-2: destruct (@LustreTiming.raw_to_comb_aux LustreTiming.TInt (@expr_to_raw Lustre.TInt e) new_ident_origin0 pre_binders0 pre_eqs0 init_post_eqs0 step_post_eqs0) as [[[[[[]]]]]] eqn: e_unfold.
-        3: destruct (@LustreTiming.raw_to_comb_aux Lustre.TInt (@expr_to_raw Lustre.TInt e) new_ident_origin0 pre_binders0 pre_eqs0 init_post_eqs0 step_post_eqs0) as [[[[[[]]]]]] eqn: e_unfold.
+        1-2: destruct (@LustreTiming.raw_to_comb LustreTiming.TInt (@expr_to_raw Lustre.TInt e) new_ident_origin0 pre_binders0 pre_eqs0 init_post_eqs0 step_post_eqs0) as [[[[[[]]]]]] eqn: e_unfold.
+        3: destruct (@LustreTiming.raw_to_comb Lustre.TInt (@expr_to_raw Lustre.TInt e) new_ident_origin0 pre_binders0 pre_eqs0 init_post_eqs0 step_post_eqs0) as [[[[[[]]]]]] eqn: e_unfold.
         all: injection eqe as <- <- <- <- <- <- <-.
         1-2: refine (IHe _ _ _ _ _ _ _ _ _ _ _ _ _ _ _ e_unfold IHn_body).
         simpl.
@@ -419,26 +459,26 @@ Proof.
           do 2 apply incl_tl.
           apply incl_refl.
       * destruct b.
-        all: unfold translate_expr_aux in eqe.
+        all: unfold translate_expr in eqe.
         all: simpl in eqe.
-        1-3: destruct (@LustreTiming.raw_to_comb_aux LustreTiming.TBool (@expr_to_raw Lustre.TBool e1) new_ident_origin0 pre_binders0 pre_eqs0 init_post_eqs0 step_post_eqs0) as [[[[[[c1 c2] ident_e1] binders_e1] eqs_e1] init_e1] step_e1] eqn: e1_unfold.
-        1-3: destruct (@LustreTiming.raw_to_comb_aux LustreTiming.TBool (@expr_to_raw Lustre.TBool e2) ident_e1 binders_e1 eqs_e1 init_e1 step_e1) as [[[[[[]]]]]] eqn: e2_unfold.
-        4-13: destruct (@LustreTiming.raw_to_comb_aux LustreTiming.TInt (@expr_to_raw Lustre.TInt e1) new_ident_origin0 pre_binders0 pre_eqs0 init_post_eqs0 step_post_eqs0) as [[[[[[c1 c2] ident_e1] binders_e1] eqs_e1] init_e1] step_e1] eqn: e1_unfold.
-        4-13: destruct (@LustreTiming.raw_to_comb_aux LustreTiming.TInt (@expr_to_raw Lustre.TInt e2) ident_e1 binders_e1 eqs_e1 init_e1 step_e1) as [[[[[[]]]]]] eqn: e2_unfold.
+        1-3: destruct (@LustreTiming.raw_to_comb LustreTiming.TBool (@expr_to_raw Lustre.TBool e1) new_ident_origin0 pre_binders0 pre_eqs0 init_post_eqs0 step_post_eqs0) as [[[[[[c1 c2] ident_e1] binders_e1] eqs_e1] init_e1] step_e1] eqn: e1_unfold.
+        1-3: destruct (@LustreTiming.raw_to_comb LustreTiming.TBool (@expr_to_raw Lustre.TBool e2) ident_e1 binders_e1 eqs_e1 init_e1 step_e1) as [[[[[[]]]]]] eqn: e2_unfold.
+        4-13: destruct (@LustreTiming.raw_to_comb LustreTiming.TInt (@expr_to_raw Lustre.TInt e1) new_ident_origin0 pre_binders0 pre_eqs0 init_post_eqs0 step_post_eqs0) as [[[[[[c1 c2] ident_e1] binders_e1] eqs_e1] init_e1] step_e1] eqn: e1_unfold.
+        4-13: destruct (@LustreTiming.raw_to_comb LustreTiming.TInt (@expr_to_raw Lustre.TInt e2) ident_e1 binders_e1 eqs_e1 init_e1 step_e1) as [[[[[[]]]]]] eqn: e2_unfold.
         1-13: injection eqe as <- <- <- <- <- <- <-.
         1-13: refine (IHe2 _ _ _ _ _ _ _ _ _ _ _ _ _ _ _ e2_unfold (IHe1 _ _ _ _ _ _ _ _ _ _ _ _ _ _ _ e1_unfold IHn_body)).
 
-        destruct (@LustreTiming.raw_to_comb_aux Lustre.TInt (@expr_to_raw Lustre.TInt e1) new_ident_origin0 pre_binders0 pre_eqs0 init_post_eqs0 step_post_eqs0) as [[[[[[c1 c2] ident_e1] binders_e1] eqs_e1] init_e1] step_e1] eqn: e1_unfold.
-        destruct (@LustreTiming.raw_to_comb_aux Lustre.TInt (@expr_to_raw Lustre.TInt e2) ident_e1 binders_e1 eqs_e1 init_e1 step_e1) as [[[[[[]]]]]] eqn: e2_unfold.
+        destruct (@LustreTiming.raw_to_comb Lustre.TInt (@expr_to_raw Lustre.TInt e1) new_ident_origin0 pre_binders0 pre_eqs0 init_post_eqs0 step_post_eqs0) as [[[[[[c1 c2] ident_e1] binders_e1] eqs_e1] init_e1] step_e1] eqn: e1_unfold.
+        destruct (@LustreTiming.raw_to_comb Lustre.TInt (@expr_to_raw Lustre.TInt e2) ident_e1 binders_e1 eqs_e1 init_e1 step_e1) as [[[[[[]]]]]] eqn: e2_unfold.
         injection eqe as <- <- <- <- <- <- <-.
         simpl.
         specialize (IHe2 _ _ _ _ _ _ _ _ _ _ _ _ _ _ _ e2_unfold (IHe1 _ _ _ _ _ _ _ _ _ _ _ _ _ _ _ e1_unfold IHn_body)).
         apply IHe2.
-      * unfold translate_expr_aux in eqe.
+      * unfold translate_expr in eqe.
         simpl in eqe.
-        destruct (@LustreTiming.raw_to_comb_aux LustreTiming.TBool (@expr_to_raw Lustre.TBool e1) new_ident_origin0 pre_binders0 pre_eqs0 init_post_eqs0 step_post_eqs0) as [[[[[[? ?] ident_e1] binders_e1] eqs_e1] init_e1] step_e1] eqn: e1_unfold.
-        destruct (@LustreTiming.raw_to_comb_aux t (@expr_to_raw t e2) ident_e1 binders_e1 eqs_e1 init_e1 step_e1) as [[[[[[? ?] ident_e2] binders_e2] eqs_e2] init_e2] step_e2] eqn: e2_unfold.
-        destruct (@LustreTiming.raw_to_comb_aux t (@expr_to_raw t e3) ident_e2 binders_e2 eqs_e2 init_e2 step_e2) as [[[[[[]]]]]] eqn: e3_unfold.
+        destruct (@LustreTiming.raw_to_comb LustreTiming.TBool (@expr_to_raw Lustre.TBool e1) new_ident_origin0 pre_binders0 pre_eqs0 init_post_eqs0 step_post_eqs0) as [[[[[[? ?] ident_e1] binders_e1] eqs_e1] init_e1] step_e1] eqn: e1_unfold.
+        destruct (@LustreTiming.raw_to_comb t (@expr_to_raw t e2) ident_e1 binders_e1 eqs_e1 init_e1 step_e1) as [[[[[[? ?] ident_e2] binders_e2] eqs_e2] init_e2] step_e2] eqn: e2_unfold.
+        destruct (@LustreTiming.raw_to_comb t (@expr_to_raw t e3) ident_e2 binders_e2 eqs_e2 init_e2 step_e2) as [[[[[[]]]]]] eqn: e3_unfold.
         injection eqe as <- <- <- <- <- <- <-.
         refine (IHe3 _ _ _ _ _ _ _ _ _ _ _ _ _ _ _ e3_unfold (IHe2 _ _ _ _ _ _ _ _ _ _ _ _ _ _ _ e2_unfold (IHe1 _ _ _ _ _ _ _ _ _ _ _ _ _ _ _ e1_unfold IHn_body))). *)
   - apply ABORT_FIXME; exact tt.
@@ -459,7 +499,7 @@ Proof.
       specialize (IHn_body incl_nbody _ _ _ _ _ _ _ _ eqIh).
       unfold Lustre.equation_dest, fst, snd, projT1 in ina.
       clear -translation IHn_body ina.
-      destruct (translate_expr_aux e new_ident_origin0 pre_binders0 pre_eqs0 init_post_eqs0 step_post_eqs0) as [[[[[[ei es] orig] binders] equations_pre] init_equations_post] step_equations_post] eqn: eqe.
+      destruct (translate_expr e new_ident_origin0 pre_binders0 pre_eqs0 init_post_eqs0 step_post_eqs0) as [[[[[[ei es] orig] binders] equations_pre] init_equations_post] step_equations_post] eqn: eqe.
       injection translation as <- <- <- <- <- <- <-.
 
       simpl.
@@ -483,10 +523,10 @@ Proof.
         assumption.
       * simpl.
         destruct u.
-        all: unfold translate_expr_aux in eqe.
+        all: unfold translate_expr in eqe.
         all: simpl in eqe.
-        1-2: destruct (@LustreTiming.raw_to_comb_aux LustreTiming.TInt (@expr_to_raw Lustre.TInt e) new_ident_origin0 pre_binders0 pre_eqs0 init_post_eqs0 step_post_eqs0) as [[[[[[]]]]]] eqn: e_unfold.
-        3: destruct (@LustreTiming.raw_to_comb_aux Lustre.TInt (@expr_to_raw Lustre.TInt e) new_ident_origin0 pre_binders0 pre_eqs0 init_post_eqs0 step_post_eqs0) as [[[[[[]]]]]] eqn: e_unfold.
+        1-2: destruct (@LustreTiming.raw_to_comb LustreTiming.TInt (@expr_to_raw Lustre.TInt e) new_ident_origin0 pre_binders0 pre_eqs0 init_post_eqs0 step_post_eqs0) as [[[[[[]]]]]] eqn: e_unfold.
+        3: destruct (@LustreTiming.raw_to_comb Lustre.TInt (@expr_to_raw Lustre.TInt e) new_ident_origin0 pre_binders0 pre_eqs0 init_post_eqs0 step_post_eqs0) as [[[[[[]]]]]] eqn: e_unfold.
         all: injection eqe as <- <- <- <- <- <- <-.
         1-2: refine (IHe _ _ _ _ _ _ _ _ _ _ _ _ _ _ _ _ e_unfold IHn_body).
         simpl.
@@ -521,17 +561,17 @@ Proof.
               apply incl_refl.
       * simpl.
         destruct b.
-        all: unfold translate_expr_aux in eqe.
+        all: unfold translate_expr in eqe.
         all: simpl in eqe.
-        1-3: destruct (@LustreTiming.raw_to_comb_aux LustreTiming.TBool (@expr_to_raw Lustre.TBool e1) new_ident_origin0 pre_binders0 pre_eqs0 init_post_eqs0 step_post_eqs0) as [[[[[[c1 c2] ident_e1] binders_e1] eqs_e1] init_e1] step_e1] eqn: e1_unfold.
-        1-3: destruct (@LustreTiming.raw_to_comb_aux LustreTiming.TBool (@expr_to_raw Lustre.TBool e2) ident_e1 binders_e1 eqs_e1 init_e1 step_e1) as [[[[[[]]]]]] eqn: e2_unfold.
-        4-13: destruct (@LustreTiming.raw_to_comb_aux LustreTiming.TInt (@expr_to_raw Lustre.TInt e1) new_ident_origin0 pre_binders0 pre_eqs0 init_post_eqs0 step_post_eqs0) as [[[[[[c1 c2] ident_e1] binders_e1] eqs_e1] init_e1] step_e1] eqn: e1_unfold.
-        4-13: destruct (@LustreTiming.raw_to_comb_aux LustreTiming.TInt (@expr_to_raw Lustre.TInt e2) ident_e1 binders_e1 eqs_e1 init_e1 step_e1) as [[[[[[]]]]]] eqn: e2_unfold.
+        1-3: destruct (@LustreTiming.raw_to_comb LustreTiming.TBool (@expr_to_raw Lustre.TBool e1) new_ident_origin0 pre_binders0 pre_eqs0 init_post_eqs0 step_post_eqs0) as [[[[[[c1 c2] ident_e1] binders_e1] eqs_e1] init_e1] step_e1] eqn: e1_unfold.
+        1-3: destruct (@LustreTiming.raw_to_comb LustreTiming.TBool (@expr_to_raw Lustre.TBool e2) ident_e1 binders_e1 eqs_e1 init_e1 step_e1) as [[[[[[]]]]]] eqn: e2_unfold.
+        4-13: destruct (@LustreTiming.raw_to_comb LustreTiming.TInt (@expr_to_raw Lustre.TInt e1) new_ident_origin0 pre_binders0 pre_eqs0 init_post_eqs0 step_post_eqs0) as [[[[[[c1 c2] ident_e1] binders_e1] eqs_e1] init_e1] step_e1] eqn: e1_unfold.
+        4-13: destruct (@LustreTiming.raw_to_comb LustreTiming.TInt (@expr_to_raw Lustre.TInt e2) ident_e1 binders_e1 eqs_e1 init_e1 step_e1) as [[[[[[]]]]]] eqn: e2_unfold.
         1-13: injection eqe as <- <- <- <- <- <- <-.
         1-13: refine (IHe2 _ _ _ _ _ _ _ _ _ _ _ _ _ _ _ _ e2_unfold (IHe1 _ _ _ _ _ _ _ _ _ _ _ _ _ _ _ _ e1_unfold IHn_body)).
 
-        destruct (@LustreTiming.raw_to_comb_aux Lustre.TInt (@expr_to_raw Lustre.TInt e1) new_ident_origin0 pre_binders0 pre_eqs0 init_post_eqs0 step_post_eqs0) as [[[[[[c1 c2] ident_e1] binders_e1] eqs_e1] init_e1] step_e1] eqn: e1_unfold.
-        destruct (@LustreTiming.raw_to_comb_aux Lustre.TInt (@expr_to_raw Lustre.TInt e2) ident_e1 binders_e1 eqs_e1 init_e1 step_e1) as [[[[[[]]]]]] eqn: e2_unfold.
+        destruct (@LustreTiming.raw_to_comb Lustre.TInt (@expr_to_raw Lustre.TInt e1) new_ident_origin0 pre_binders0 pre_eqs0 init_post_eqs0 step_post_eqs0) as [[[[[[c1 c2] ident_e1] binders_e1] eqs_e1] init_e1] step_e1] eqn: e1_unfold.
+        destruct (@LustreTiming.raw_to_comb Lustre.TInt (@expr_to_raw Lustre.TInt e2) ident_e1 binders_e1 eqs_e1 init_e1 step_e1) as [[[[[[]]]]]] eqn: e2_unfold.
         injection eqe as <- <- <- <- <- <- <-.
         simpl.
         specialize (IHe2 _ _ _ _ _ _ _ _ _ _ _ _ _ _ _ _ e2_unfold (IHe1 _ _ _ _ _ _ _ _ _ _ _ _ _ _ _ _ e1_unfold IHn_body)).
@@ -549,11 +589,11 @@ Proof.
         ++ apply incl_app_inv in IHe2.
           destruct IHe2 as [_ incl_l1].
           apply incl_l1.
-      * unfold translate_expr_aux in eqe.
+      * unfold translate_expr in eqe.
         simpl in eqe.
-        destruct (@LustreTiming.raw_to_comb_aux LustreTiming.TBool (@expr_to_raw Lustre.TBool e1) new_ident_origin0 pre_binders0 pre_eqs0 init_post_eqs0 step_post_eqs0) as [[[[[[? ?] ident_e1] binders_e1] eqs_e1] init_e1] step_e1] eqn: e1_unfold.
-        destruct (@LustreTiming.raw_to_comb_aux t (@expr_to_raw t e2) ident_e1 binders_e1 eqs_e1 init_e1 step_e1) as [[[[[[? ?] ident_e2] binders_e2] eqs_e2] init_e2] step_e2] eqn: e2_unfold.
-        destruct (@LustreTiming.raw_to_comb_aux t (@expr_to_raw t e3) ident_e2 binders_e2 eqs_e2 init_e2 step_e2) as [[[[[[]]]]]] eqn: e3_unfold.
+        destruct (@LustreTiming.raw_to_comb LustreTiming.TBool (@expr_to_raw Lustre.TBool e1) new_ident_origin0 pre_binders0 pre_eqs0 init_post_eqs0 step_post_eqs0) as [[[[[[? ?] ident_e1] binders_e1] eqs_e1] init_e1] step_e1] eqn: e1_unfold.
+        destruct (@LustreTiming.raw_to_comb t (@expr_to_raw t e2) ident_e1 binders_e1 eqs_e1 init_e1 step_e1) as [[[[[[? ?] ident_e2] binders_e2] eqs_e2] init_e2] step_e2] eqn: e2_unfold.
+        destruct (@LustreTiming.raw_to_comb t (@expr_to_raw t e3) ident_e2 binders_e2 eqs_e2 init_e2 step_e2) as [[[[[[]]]]]] eqn: e3_unfold.
         injection eqe as <- <- <- <- <- <- <-.
         refine (IHe3 _ _ _ _ _ _ _ _ _ _ _ _ _ _ _ _ e3_unfold (IHe2 _ _ _ _ _ _ _ _ _ _ _ _ _ _ _ _ e2_unfold (IHe1 _ _ _ _ _ _ _ _ _ _ _ _ _ _ _ _ e1_unfold IHn_body))). *)
   - apply ABORT_FIXME; exact tt.
@@ -571,7 +611,7 @@ Proof.
     simpl in translation.
     destruct (translate_equations n_body ident_origin) as [[[[[[init_eq step_eq] origin_ident] binders_pre] equations_pre] post_init_equations] post_step_equations] eqn: translate_nbody.
     destruct eq as [i [ty e]].
-    destruct (translate_expr_aux e origin_ident binders_pre equations_pre post_init_equations post_step_equations) as [[[[[[]]]]]] eqn: unfold_translate.
+    destruct (translate_expr e origin_ident binders_pre equations_pre post_init_equations post_step_equations) as [[[[[[]]]]]] eqn: unfold_translate.
     injection translation as <- <- <- <- <- <- <-.
     unfold Lustre.equation_dest at 1, fst, snd, projT1 in a_assigned.
     simpl.
@@ -592,41 +632,41 @@ Proof.
     rename unfold_translate into translation.
 
     induction e in a, origin_ident, binders_pre, equations_pre, post_init_equations, post_step_equations, init_eq, step_eq, new_origin_ident, new_binders_pre, new_equations_pre, new_post_init_equations, new_post_step_equations, translation, in_post_init |- *.
-    1-3: unfold translate_expr_aux in translation.
+    1-3: unfold translate_expr in translation.
     1-3: simpl in translation.
     1-3: injection translation as <- <- <- <- <- <- <-.
     1-3: assumption.
 
-    + unfold translate_expr_aux in translation.
+    + unfold translate_expr in translation.
       destruct u.
       all: simpl in translation.
-      1-2: destruct (@LustreTiming.raw_to_comb_aux LustreTiming.TInt (@expr_to_raw Lustre.TInt e) origin_ident binders_pre equations_pre post_init_equations post_step_equations) as [[[[[[]]]]]] eqn: unfold_e.
+      1-2: destruct (@LustreTiming.raw_to_comb LustreTiming.TInt (@expr_to_raw Lustre.TInt e) origin_ident binders_pre equations_pre post_init_equations post_step_equations) as [[[[[[]]]]]] eqn: unfold_e.
       1-2: injection translation as <- <- <- <- <- <- <-.
       1-2: refine (IHe _ _ _ _ _ _ _ _ _ _ _ _ _ unfold_e in_post_init).
 
-      destruct (@LustreTiming.raw_to_comb_aux Lustre.TInt (@expr_to_raw Lustre.TInt e) origin_ident binders_pre equations_pre post_init_equations post_step_equations) as [[[[[[]]]]]] eqn: unfold_e.
+      destruct (@LustreTiming.raw_to_comb Lustre.TInt (@expr_to_raw Lustre.TInt e) origin_ident binders_pre equations_pre post_init_equations post_step_equations) as [[[[[[]]]]]] eqn: unfold_e.
 
       injection translation as <- <- <- <- <- <- <-.
       specialize (IHe _ _ _ _ _ _ _ _ _ _ _ _ _ unfold_e in_post_init).
       simpl.
       right.
       assumption.
-    + unfold translate_expr_aux in translation.
+    + unfold translate_expr in translation.
       destruct b.
       all: simpl in translation.
-      1-3: destruct (@LustreTiming.raw_to_comb_aux LustreTiming.TBool (@expr_to_raw Lustre.TBool e1) origin_ident binders_pre equations_pre post_init_equations post_step_equations) as [[[[[[c1 c2] ident_e1] binders_e1] eqs_e1] init_e1] step_e1] eqn: e1_unfold.
-      1-3: destruct (@LustreTiming.raw_to_comb_aux LustreTiming.TBool (@expr_to_raw Lustre.TBool e2) ident_e1 binders_e1 eqs_e1 init_e1 step_e1) as [[[[[[]]]]]] eqn: e2_unfold.
-      4-13: destruct (@LustreTiming.raw_to_comb_aux LustreTiming.TInt (@expr_to_raw Lustre.TInt e1) origin_ident binders_pre equations_pre post_init_equations post_step_equations) as [[[[[[c1 c2] ident_e1] binders_e1] eqs_e1] init_e1] step_e1] eqn: e1_unfold.
-      4-13: destruct (@LustreTiming.raw_to_comb_aux LustreTiming.TInt (@expr_to_raw Lustre.TInt e2) ident_e1 binders_e1 eqs_e1 init_e1 step_e1) as [[[[[[]]]]]] eqn: e2_unfold.
-      14: destruct (@LustreTiming.raw_to_comb_aux Lustre.TInt (@expr_to_raw Lustre.TInt e1) origin_ident binders_pre equations_pre post_init_equations post_step_equations) as [[[[[[c1 c2] ident_e1] binders_e1] eqs_e1] init_e1] step_e1] eqn: e1_unfold.
-      14: destruct (@LustreTiming.raw_to_comb_aux Lustre.TInt (@expr_to_raw Lustre.TInt e2) ident_e1 binders_e1 eqs_e1 init_e1 step_e1) as [[[[[[]]]]]] eqn: e2_unfold.
+      1-3: destruct (@LustreTiming.raw_to_comb LustreTiming.TBool (@expr_to_raw Lustre.TBool e1) origin_ident binders_pre equations_pre post_init_equations post_step_equations) as [[[[[[c1 c2] ident_e1] binders_e1] eqs_e1] init_e1] step_e1] eqn: e1_unfold.
+      1-3: destruct (@LustreTiming.raw_to_comb LustreTiming.TBool (@expr_to_raw Lustre.TBool e2) ident_e1 binders_e1 eqs_e1 init_e1 step_e1) as [[[[[[]]]]]] eqn: e2_unfold.
+      4-13: destruct (@LustreTiming.raw_to_comb LustreTiming.TInt (@expr_to_raw Lustre.TInt e1) origin_ident binders_pre equations_pre post_init_equations post_step_equations) as [[[[[[c1 c2] ident_e1] binders_e1] eqs_e1] init_e1] step_e1] eqn: e1_unfold.
+      4-13: destruct (@LustreTiming.raw_to_comb LustreTiming.TInt (@expr_to_raw Lustre.TInt e2) ident_e1 binders_e1 eqs_e1 init_e1 step_e1) as [[[[[[]]]]]] eqn: e2_unfold.
+      14: destruct (@LustreTiming.raw_to_comb Lustre.TInt (@expr_to_raw Lustre.TInt e1) origin_ident binders_pre equations_pre post_init_equations post_step_equations) as [[[[[[c1 c2] ident_e1] binders_e1] eqs_e1] init_e1] step_e1] eqn: e1_unfold.
+      14: destruct (@LustreTiming.raw_to_comb Lustre.TInt (@expr_to_raw Lustre.TInt e2) ident_e1 binders_e1 eqs_e1 init_e1 step_e1) as [[[[[[]]]]]] eqn: e2_unfold.
       all: injection translation as <- <- <- <- <- <- <-.
       all: refine (IHe2 _ _ _ _ _ _ _ _ _ _ _ _ _ e2_unfold (IHe1 _ _ _ _ _ _ _ _ _ _ _ _ _ e1_unfold in_post_init)).
-    + unfold translate_expr_aux in translation.
+    + unfold translate_expr in translation.
       simpl in translation.
-      destruct (@LustreTiming.raw_to_comb_aux LustreTiming.TBool (@expr_to_raw Lustre.TBool e1) origin_ident binders_pre equations_pre post_init_equations post_step_equations) as [[[[[[? ?] ident_e1] binders_e1] eqs_e1] init_e1] step_e1] eqn: e1_unfold.
-      destruct (@LustreTiming.raw_to_comb_aux t (@expr_to_raw t e2) ident_e1 binders_e1 eqs_e1 init_e1 step_e1) as [[[[[[? ?] ident_e2] binders_e2] eqs_e2] init_e2] step_e2] eqn: e2_unfold.
-      destruct (@LustreTiming.raw_to_comb_aux t (@expr_to_raw t e3) ident_e2 binders_e2 eqs_e2 init_e2 step_e2) as [[[[[[]]]]]] eqn: e3_unfold.
+      destruct (@LustreTiming.raw_to_comb LustreTiming.TBool (@expr_to_raw Lustre.TBool e1) origin_ident binders_pre equations_pre post_init_equations post_step_equations) as [[[[[[? ?] ident_e1] binders_e1] eqs_e1] init_e1] step_e1] eqn: e1_unfold.
+      destruct (@LustreTiming.raw_to_comb t (@expr_to_raw t e2) ident_e1 binders_e1 eqs_e1 init_e1 step_e1) as [[[[[[? ?] ident_e2] binders_e2] eqs_e2] init_e2] step_e2] eqn: e2_unfold.
+      destruct (@LustreTiming.raw_to_comb t (@expr_to_raw t e3) ident_e2 binders_e2 eqs_e2 init_e2 step_e2) as [[[[[[]]]]]] eqn: e3_unfold.
       injection translation as <- <- <- <- <- <- <-.
       refine (IHe3 _ _ _ _ _ _ _ _ _ _ _ _ _ e3_unfold (IHe2 _ _ _ _ _ _ _ _ _ _ _ _ _ e2_unfold (IHe1 _ _ _ _ _ _ _ _ _ _ _ _ _ e1_unfold in_post_init))). *)
   - apply ABORT_FIXME; exact tt.
@@ -645,7 +685,7 @@ Proof.
     simpl in translation.
     destruct (translate_equations n_body ident_origin) as [[[[[[init_eq step_eq] origin_ident] binders_pre] equations_pre] post_init_equations] post_step_equations] eqn: translate_nbody.
     destruct eq as [i [ty e]].
-    destruct (translate_expr_aux e origin_ident binders_pre equations_pre post_init_equations post_step_equations) as [[[[[[]]]]]] eqn: unfold_translate.
+    destruct (translate_expr e origin_ident binders_pre equations_pre post_init_equations post_step_equations) as [[[[[[]]]]]] eqn: unfold_translate.
     injection translation as <- <- <- <- <- <- <-.
     unfold Lustre.equation_dest at 1, fst, snd, projT1 in a_assigned.
     simpl.
@@ -664,41 +704,41 @@ Proof.
     rename unfold_translate into translation.
 
     induction e in a, origin_ident, binders_pre, equations_pre, post_init_equations, post_step_equations, init_eq, step_eq, new_origin_ident, new_binders_pre, new_equations_pre, new_post_init_equations, new_post_step_equations, translation, in_post_init |- *.
-    1-3: unfold translate_expr_aux in translation.
+    1-3: unfold translate_expr in translation.
     1-3: simpl in translation.
     1-3: injection translation as <- <- <- <- <- <- <-.
     1-3: assumption.
 
-    + unfold translate_expr_aux in translation.
+    + unfold translate_expr in translation.
       destruct u.
       all: simpl in translation.
-      1-2: destruct (@LustreTiming.raw_to_comb_aux LustreTiming.TInt (@expr_to_raw Lustre.TInt e) origin_ident binders_pre equations_pre post_init_equations post_step_equations) as [[[[[[]]]]]] eqn: unfold_e.
+      1-2: destruct (@LustreTiming.raw_to_comb LustreTiming.TInt (@expr_to_raw Lustre.TInt e) origin_ident binders_pre equations_pre post_init_equations post_step_equations) as [[[[[[]]]]]] eqn: unfold_e.
       1-2: injection translation as <- <- <- <- <- <- <-.
       1-2: refine (IHe _ _ _ _ _ _ _ _ _ _ _ _ _ unfold_e in_post_init).
 
-      destruct (@LustreTiming.raw_to_comb_aux Lustre.TInt (@expr_to_raw Lustre.TInt e) origin_ident binders_pre equations_pre post_init_equations post_step_equations) as [[[[[[]]]]]] eqn: unfold_e.
+      destruct (@LustreTiming.raw_to_comb Lustre.TInt (@expr_to_raw Lustre.TInt e) origin_ident binders_pre equations_pre post_init_equations post_step_equations) as [[[[[[]]]]]] eqn: unfold_e.
 
       injection translation as <- <- <- <- <- <- <-.
       specialize (IHe _ _ _ _ _ _ _ _ _ _ _ _ _ unfold_e in_post_init).
       simpl.
       right.
       assumption.
-    + unfold translate_expr_aux in translation.
+    + unfold translate_expr in translation.
       destruct b.
       all: simpl in translation.
-      1-3: destruct (@LustreTiming.raw_to_comb_aux LustreTiming.TBool (@expr_to_raw Lustre.TBool e1) origin_ident binders_pre equations_pre post_init_equations post_step_equations) as [[[[[[c1 c2] ident_e1] binders_e1] eqs_e1] init_e1] step_e1] eqn: e1_unfold.
-      1-3: destruct (@LustreTiming.raw_to_comb_aux LustreTiming.TBool (@expr_to_raw Lustre.TBool e2) ident_e1 binders_e1 eqs_e1 init_e1 step_e1) as [[[[[[]]]]]] eqn: e2_unfold.
-      4-13: destruct (@LustreTiming.raw_to_comb_aux LustreTiming.TInt (@expr_to_raw Lustre.TInt e1) origin_ident binders_pre equations_pre post_init_equations post_step_equations) as [[[[[[c1 c2] ident_e1] binders_e1] eqs_e1] init_e1] step_e1] eqn: e1_unfold.
-      4-13: destruct (@LustreTiming.raw_to_comb_aux LustreTiming.TInt (@expr_to_raw Lustre.TInt e2) ident_e1 binders_e1 eqs_e1 init_e1 step_e1) as [[[[[[]]]]]] eqn: e2_unfold.
-      14: destruct (@LustreTiming.raw_to_comb_aux Lustre.TInt (@expr_to_raw Lustre.TInt e1) origin_ident binders_pre equations_pre post_init_equations post_step_equations) as [[[[[[c1 c2] ident_e1] binders_e1] eqs_e1] init_e1] step_e1] eqn: e1_unfold.
-      14: destruct (@LustreTiming.raw_to_comb_aux Lustre.TInt (@expr_to_raw Lustre.TInt e2) ident_e1 binders_e1 eqs_e1 init_e1 step_e1) as [[[[[[]]]]]] eqn: e2_unfold.
+      1-3: destruct (@LustreTiming.raw_to_comb LustreTiming.TBool (@expr_to_raw Lustre.TBool e1) origin_ident binders_pre equations_pre post_init_equations post_step_equations) as [[[[[[c1 c2] ident_e1] binders_e1] eqs_e1] init_e1] step_e1] eqn: e1_unfold.
+      1-3: destruct (@LustreTiming.raw_to_comb LustreTiming.TBool (@expr_to_raw Lustre.TBool e2) ident_e1 binders_e1 eqs_e1 init_e1 step_e1) as [[[[[[]]]]]] eqn: e2_unfold.
+      4-13: destruct (@LustreTiming.raw_to_comb LustreTiming.TInt (@expr_to_raw Lustre.TInt e1) origin_ident binders_pre equations_pre post_init_equations post_step_equations) as [[[[[[c1 c2] ident_e1] binders_e1] eqs_e1] init_e1] step_e1] eqn: e1_unfold.
+      4-13: destruct (@LustreTiming.raw_to_comb LustreTiming.TInt (@expr_to_raw Lustre.TInt e2) ident_e1 binders_e1 eqs_e1 init_e1 step_e1) as [[[[[[]]]]]] eqn: e2_unfold.
+      14: destruct (@LustreTiming.raw_to_comb Lustre.TInt (@expr_to_raw Lustre.TInt e1) origin_ident binders_pre equations_pre post_init_equations post_step_equations) as [[[[[[c1 c2] ident_e1] binders_e1] eqs_e1] init_e1] step_e1] eqn: e1_unfold.
+      14: destruct (@LustreTiming.raw_to_comb Lustre.TInt (@expr_to_raw Lustre.TInt e2) ident_e1 binders_e1 eqs_e1 init_e1 step_e1) as [[[[[[]]]]]] eqn: e2_unfold.
       all: injection translation as <- <- <- <- <- <- <-.
       all: refine (IHe2 _ _ _ _ _ _ _ _ _ _ _ _ _ e2_unfold (IHe1 _ _ _ _ _ _ _ _ _ _ _ _ _ e1_unfold in_post_init)).
-    + unfold translate_expr_aux in translation.
+    + unfold translate_expr in translation.
       simpl in translation.
-      destruct (@LustreTiming.raw_to_comb_aux LustreTiming.TBool (@expr_to_raw Lustre.TBool e1) origin_ident binders_pre equations_pre post_init_equations post_step_equations) as [[[[[[? ?] ident_e1] binders_e1] eqs_e1] init_e1] step_e1] eqn: e1_unfold.
-      destruct (@LustreTiming.raw_to_comb_aux t (@expr_to_raw t e2) ident_e1 binders_e1 eqs_e1 init_e1 step_e1) as [[[[[[? ?] ident_e2] binders_e2] eqs_e2] init_e2] step_e2] eqn: e2_unfold.
-      destruct (@LustreTiming.raw_to_comb_aux t (@expr_to_raw t e3) ident_e2 binders_e2 eqs_e2 init_e2 step_e2) as [[[[[[]]]]]] eqn: e3_unfold.
+      destruct (@LustreTiming.raw_to_comb LustreTiming.TBool (@expr_to_raw Lustre.TBool e1) origin_ident binders_pre equations_pre post_init_equations post_step_equations) as [[[[[[? ?] ident_e1] binders_e1] eqs_e1] init_e1] step_e1] eqn: e1_unfold.
+      destruct (@LustreTiming.raw_to_comb t (@expr_to_raw t e2) ident_e1 binders_e1 eqs_e1 init_e1 step_e1) as [[[[[[? ?] ident_e2] binders_e2] eqs_e2] init_e2] step_e2] eqn: e2_unfold.
+      destruct (@LustreTiming.raw_to_comb t (@expr_to_raw t e3) ident_e2 binders_e2 eqs_e2 init_e2 step_e2) as [[[[[[]]]]]] eqn: e3_unfold.
       injection translation as <- <- <- <- <- <- <-.
       refine (IHe3 _ _ _ _ _ _ _ _ _ _ _ _ _ e3_unfold (IHe2 _ _ _ _ _ _ _ _ _ _ _ _ _ e2_unfold (IHe1 _ _ _ _ _ _ _ _ _ _ _ _ _ e1_unfold in_post_init))). *)
 
@@ -721,7 +761,7 @@ Proof.
     simpl in translation.
     destruct (translate_equations n_body ident_origin) as [[[[[[init_eq step_eq] origin_ident] binders_pre] equations_pre] post_init_equations] post_step_equations] eqn: translate_nbody.
     destruct eq as [i [ty e]].
-    destruct (translate_expr_aux e origin_ident binders_pre equations_pre post_init_equations post_step_equations) as [[[[[[ei es] new_orig_ident] new_binders_pre] new_eqs_pre] new_init_eqs] new_step_eqs] eqn: unfold_translate.
+    destruct (translate_expr e origin_ident binders_pre equations_pre post_init_equations post_step_equations) as [[[[[[ei es] new_orig_ident] new_binders_pre] new_eqs_pre] new_init_eqs] new_step_eqs] eqn: unfold_translate.
     injection translation as <- <- <- <- <- <- <-.
     simpl.
     rename unfold_translate into translation.
@@ -731,7 +771,7 @@ Proof.
       injection a_is_eq as <- <-.
       apply Lustre.sig2T_eq_type in H.
       subst.
-      unfold translate_expr_aux in translation.
+      unfold translate_expr in translation.
       simpl in translation.
       injection translation as <- <- <- <- <- <-.
       reflexivity.
@@ -745,41 +785,41 @@ Proof.
       clear -translation in_post_init.
 
       induction e in name, tya, origin_ident, binders_pre, equations_pre, new_orig_ident, new_binders_pre, new_eqs_pre, new_init_eqs, new_step_eqs, translation, in_post_init, post_init_equations, post_step_equations, ei, es |- *.
-      1-3: unfold translate_expr_aux in translation.
+      1-3: unfold translate_expr in translation.
       1-3: simpl in translation.
       1-3: injection translation as <- <- <- <- <- <- <-.
       1-3: assumption.
 
-      * unfold translate_expr_aux in translation.
+      * unfold translate_expr in translation.
         destruct u.
         all: simpl in translation.
-        1-2: destruct (@LustreTiming.raw_to_comb_aux LustreTiming.TInt (@expr_to_raw Lustre.TInt e) origin_ident binders_pre equations_pre post_init_equations post_step_equations) as [[[[[[]]]]]] eqn: unfold_e.
+        1-2: destruct (@LustreTiming.raw_to_comb LustreTiming.TInt (@expr_to_raw Lustre.TInt e) origin_ident binders_pre equations_pre post_init_equations post_step_equations) as [[[[[[]]]]]] eqn: unfold_e.
         1-2: injection translation as <- <- <- <- <- <- <-.
         1-2: refine (IHe _ _ _ _ _ _ _ _ _ _ _ _ _ _ unfold_e in_post_init).
 
-        destruct (@LustreTiming.raw_to_comb_aux Lustre.TInt (@expr_to_raw Lustre.TInt e) origin_ident binders_pre equations_pre post_init_equations post_step_equations) as [[[[[[]]]]]] eqn: unfold_e.
+        destruct (@LustreTiming.raw_to_comb Lustre.TInt (@expr_to_raw Lustre.TInt e) origin_ident binders_pre equations_pre post_init_equations post_step_equations) as [[[[[[]]]]]] eqn: unfold_e.
 
         injection translation as <- <- <- <- <- <- <-.
         specialize (IHe _ _ _ _ _ _ _ _ _ _ _ _ _ _ unfold_e in_post_init).
         simpl.
         right.
         assumption.
-      * unfold translate_expr_aux in translation.
+      * unfold translate_expr in translation.
         destruct b.
         all: simpl in translation.
-        1-3: destruct (@LustreTiming.raw_to_comb_aux LustreTiming.TBool (@expr_to_raw Lustre.TBool e1) origin_ident binders_pre equations_pre post_init_equations post_step_equations) as [[[[[[c1 c2] ident_e1] binders_e1] eqs_e1] init_e1] step_e1] eqn: e1_unfold.
-        1-3: destruct (@LustreTiming.raw_to_comb_aux LustreTiming.TBool (@expr_to_raw Lustre.TBool e2) ident_e1 binders_e1 eqs_e1 init_e1 step_e1) as [[[[[[]]]]]] eqn: e2_unfold.
-        4-13: destruct (@LustreTiming.raw_to_comb_aux LustreTiming.TInt (@expr_to_raw Lustre.TInt e1) origin_ident binders_pre equations_pre post_init_equations post_step_equations) as [[[[[[c1 c2] ident_e1] binders_e1] eqs_e1] init_e1] step_e1] eqn: e1_unfold.
-        4-13: destruct (@LustreTiming.raw_to_comb_aux LustreTiming.TInt (@expr_to_raw Lustre.TInt e2) ident_e1 binders_e1 eqs_e1 init_e1 step_e1) as [[[[[[]]]]]] eqn: e2_unfold.
-        14: destruct (@LustreTiming.raw_to_comb_aux Lustre.TInt (@expr_to_raw Lustre.TInt e1) origin_ident binders_pre equations_pre post_init_equations post_step_equations) as [[[[[[c1 c2] ident_e1] binders_e1] eqs_e1] init_e1] step_e1] eqn: e1_unfold.
-        14: destruct (@LustreTiming.raw_to_comb_aux Lustre.TInt (@expr_to_raw Lustre.TInt e2) ident_e1 binders_e1 eqs_e1 init_e1 step_e1) as [[[[[[]]]]]] eqn: e2_unfold.
+        1-3: destruct (@LustreTiming.raw_to_comb LustreTiming.TBool (@expr_to_raw Lustre.TBool e1) origin_ident binders_pre equations_pre post_init_equations post_step_equations) as [[[[[[c1 c2] ident_e1] binders_e1] eqs_e1] init_e1] step_e1] eqn: e1_unfold.
+        1-3: destruct (@LustreTiming.raw_to_comb LustreTiming.TBool (@expr_to_raw Lustre.TBool e2) ident_e1 binders_e1 eqs_e1 init_e1 step_e1) as [[[[[[]]]]]] eqn: e2_unfold.
+        4-13: destruct (@LustreTiming.raw_to_comb LustreTiming.TInt (@expr_to_raw Lustre.TInt e1) origin_ident binders_pre equations_pre post_init_equations post_step_equations) as [[[[[[c1 c2] ident_e1] binders_e1] eqs_e1] init_e1] step_e1] eqn: e1_unfold.
+        4-13: destruct (@LustreTiming.raw_to_comb LustreTiming.TInt (@expr_to_raw Lustre.TInt e2) ident_e1 binders_e1 eqs_e1 init_e1 step_e1) as [[[[[[]]]]]] eqn: e2_unfold.
+        14: destruct (@LustreTiming.raw_to_comb Lustre.TInt (@expr_to_raw Lustre.TInt e1) origin_ident binders_pre equations_pre post_init_equations post_step_equations) as [[[[[[c1 c2] ident_e1] binders_e1] eqs_e1] init_e1] step_e1] eqn: e1_unfold.
+        14: destruct (@LustreTiming.raw_to_comb Lustre.TInt (@expr_to_raw Lustre.TInt e2) ident_e1 binders_e1 eqs_e1 init_e1 step_e1) as [[[[[[]]]]]] eqn: e2_unfold.
         all: injection translation as <- <- <- <- <- <- <-.
         all: refine (IHe2 _ _ _ _ _ _ _ _ _ _ _ _ _ _ e2_unfold (IHe1 _ _ _ _ _ _ _ _ _ _ _ _ _ _ e1_unfold in_post_init)).
-      * unfold translate_expr_aux in translation.
+      * unfold translate_expr in translation.
         simpl in translation.
-        destruct (@LustreTiming.raw_to_comb_aux LustreTiming.TBool (@expr_to_raw Lustre.TBool e1) origin_ident binders_pre equations_pre post_init_equations post_step_equations) as [[[[[[? ?] ident_e1] binders_e1] eqs_e1] init_e1] step_e1] eqn: e1_unfold.
-        destruct (@LustreTiming.raw_to_comb_aux t (@expr_to_raw t e2) ident_e1 binders_e1 eqs_e1 init_e1 step_e1) as [[[[[[? ?] ident_e2] binders_e2] eqs_e2] init_e2] step_e2] eqn: e2_unfold.
-        destruct (@LustreTiming.raw_to_comb_aux t (@expr_to_raw t e3) ident_e2 binders_e2 eqs_e2 init_e2 step_e2) as [[[[[[]]]]]] eqn: e3_unfold.
+        destruct (@LustreTiming.raw_to_comb LustreTiming.TBool (@expr_to_raw Lustre.TBool e1) origin_ident binders_pre equations_pre post_init_equations post_step_equations) as [[[[[[? ?] ident_e1] binders_e1] eqs_e1] init_e1] step_e1] eqn: e1_unfold.
+        destruct (@LustreTiming.raw_to_comb t (@expr_to_raw t e2) ident_e1 binders_e1 eqs_e1 init_e1 step_e1) as [[[[[[? ?] ident_e2] binders_e2] eqs_e2] init_e2] step_e2] eqn: e2_unfold.
+        destruct (@LustreTiming.raw_to_comb t (@expr_to_raw t e3) ident_e2 binders_e2 eqs_e2 init_e2 step_e2) as [[[[[[]]]]]] eqn: e3_unfold.
         injection translation as <- <- <- <- <- <- <-.
         refine (IHe3 _ _ _ _ _ _ _ _ _ _ _ _ _ _ e3_unfold (IHe2 _ _ _ _ _ _ _ _ _ _ _ _ _ _ e2_unfold (IHe1 _ _ _ _ _ _ _ _ _ _ _ _ _ _ e1_unfold in_post_init))). *)
   (* EInput, will be changed later *)
